Use bounded ints in externs in BoundedIntExamples

Source/DafnyStandardLibraries/examples/BoundedIntExamples.dfy
@@ -1,15 +1,22 @@
 import opened DafnyStdLibs.BoundedInts
 
-method BoundedIntUser(x: uint32, z: nat16) {
-
-  assert TWO_TO_THE_15 * 2 == TWO_TO_THE_16;
-
-  assert 0 <= (x as int) < TWO_TO_THE_32;
+lemma BoundedIntUser(x: uint32, z: nat16)
+  ensures TWO_TO_THE_15 * 2 == TWO_TO_THE_16
+  ensures 0 <= (x as int) < TWO_TO_THE_32
+{
   var y: uint64 := x as int as uint64;
   var int16 := z as int as int16;
   var uint16 := z as int as uint16;
-  
-  // Nat can be converted to int without a cast
-  var nat234: nat16 := 234;
-  var int234 := nat234;
+}
+
+method {:test} UseExterns() {
+  var squareOf8 := Externs.NonDefault.SquareNativeInt(8);
+  expect squareOf8 == 64;
+}
+
+module {:extern} Externs {
+  import opened DafnyStdLibs.BoundedInts
+  class {:extern} NonDefault {
+    static method {:extern} SquareNativeInt(i: int32) returns (r: int32)
+  }
 }
